libcrux-ml-dsa/proofs/fstar/extraction/Libcrux_ml_dsa.Simd.Portable.Arithmetic.fsti
@@ -14,32 +14,26 @@ let v_MONTGOMERY_SHIFT: u8 = mk_u8 32
 val add (lhs rhs: Libcrux_ml_dsa.Simd.Portable.Vector_type.t_Coefficients)
     : Prims.Pure Libcrux_ml_dsa.Simd.Portable.Vector_type.t_Coefficients
       (requires
-        forall i.
-          i < 8 ==>
-          Spec.Utils.is_intb (pow2 31 - 1)
-            (v (Seq.index lhs.f_values i) + v (Seq.index rhs.f_values i)))
+        Libcrux_ml_dsa.Simd.Traits.add_pre lhs.Libcrux_ml_dsa.Simd.Portable.Vector_type.f_values
+          rhs.Libcrux_ml_dsa.Simd.Portable.Vector_type.f_values)
       (ensures
         fun lhs_future ->
           let lhs_future:Libcrux_ml_dsa.Simd.Portable.Vector_type.t_Coefficients = lhs_future in
-          forall i.
-            i < 8 ==>
-            (v (Seq.index lhs_future.f_values i) ==
-              v (Seq.index lhs.f_values i) + v (Seq.index rhs.f_values i)))
+          Libcrux_ml_dsa.Simd.Traits.add_post lhs.Libcrux_ml_dsa.Simd.Portable.Vector_type.f_values
+            rhs.Libcrux_ml_dsa.Simd.Portable.Vector_type.f_values
+            lhs_future.Libcrux_ml_dsa.Simd.Portable.Vector_type.f_values)
 
 val subtract (lhs rhs: Libcrux_ml_dsa.Simd.Portable.Vector_type.t_Coefficients)
     : Prims.Pure Libcrux_ml_dsa.Simd.Portable.Vector_type.t_Coefficients
       (requires
-        forall i.
-          i < 8 ==>
-          Spec.Utils.is_intb (pow2 31 - 1)
-            (v (Seq.index lhs.f_values i) - v (Seq.index rhs.f_values i)))
+        Libcrux_ml_dsa.Simd.Traits.sub_pre lhs.Libcrux_ml_dsa.Simd.Portable.Vector_type.f_values
+          rhs.Libcrux_ml_dsa.Simd.Portable.Vector_type.f_values)
       (ensures
         fun lhs_future ->
           let lhs_future:Libcrux_ml_dsa.Simd.Portable.Vector_type.t_Coefficients = lhs_future in
-          forall i.
-            i < 8 ==>
-            (v (Seq.index lhs_future.f_values i) ==
-              v (Seq.index lhs.f_values i) - v (Seq.index rhs.f_values i)))
+          Libcrux_ml_dsa.Simd.Traits.sub_post lhs.Libcrux_ml_dsa.Simd.Portable.Vector_type.f_values
+            rhs.Libcrux_ml_dsa.Simd.Portable.Vector_type.f_values
+            lhs_future.Libcrux_ml_dsa.Simd.Portable.Vector_type.f_values)
 
 val get_n_least_significant_bits (n: u8) (value: u64)
     : Prims.Pure u64
